src/coqutil/Map/MapKeys.v
@@ -1,13 +1,13 @@
-Require Import coqutil.Decidable coqutil.Map.Interface.
-Require coqutil.Decidable coqutil.Map.Properties.
+Require Import coqutil.Decidable coqutil.Eqb coqutil.Map.Interface.
+Require coqutil.Map.Properties.
 Import Interface.map.
 
 Module map.
   Section MapKeys. Local Set Default Proof Using "All".
     Context {key value} {map : map key value} {ok : map.ok map}.
-    Context {key_eqb: key -> key -> bool} {key_eq_dec: EqDecider key_eqb}.
+    Context {key_eqb: Eqb key} {key_eq_dec: EqDecider key_eqb}.
     Context {key'} {map' : Interface.map.map key' value} {ok' : map.ok map'}.
-    Context {key'_eqb: key' -> key' -> bool} {key'_eq_dec: EqDecider key'_eqb}.
+    Context {key'_eqb: Eqb key'} {key'_eq_dec: EqDecider key'_eqb}.
 
     Definition map_keys f (m:map) : map' := fold (fun m k v => put m (f k) v) empty m.
     Lemma get_map_keys_invertible (f : key -> key') m k
